TaplLean/Util.lean
@@ -6,10 +6,3 @@ class StepRel (α : Type u) where
   step : α → α → Prop
 
 infixr:50 " -> " => StepRel.step
-
-inductive MultiStep {α : Type u} [inst : StepRel α] : α → α → Prop where
-  | refl {t} : MultiStep t t
-  | step {t t'} (h : StepRel.step t t') : MultiStep t t'
-  | trans {t t' t''} (h₁ : MultiStep t t') (h₂ : MultiStep t' t'') : MultiStep t t''
-
-infixr:50 " ->* " => MultiStep
